Prove Poseidon2 stdlib hash specs

stdlib/lampe/Stdlib/Hash/Mod.lean
@@ -1,6 +1,248 @@
 import «std-1.0.0-beta.14».Extracted
 import Lampe
+import Stdlib.Default
 
 namespace Lampe.Stdlib.Hash
 
 open «std-1.0.0-beta.14»
+
+abbrev BuildHasherDefaultTp (H : Tp) : Tp :=
+  «std-1.0.0-beta.14::hash::BuildHasherDefault».tp h![H]
+
+abbrev Hasher.hasImpl (env : Env) (tp : Tp) :=
+  «std-1.0.0-beta.14::hash::Hasher».hasImpl env h![] tp
+
+abbrev HashTrait.hasImpl (env : Env) (tp : Tp) :=
+  «std-1.0.0-beta.14::hash::Hash».hasImpl env h![] tp
+
+def buildHasherDefaultRepr {p H} : Tp.denote p (BuildHasherDefaultTp H) :=
+  HList.toTuple p h![] (some «std-1.0.0-beta.14::hash::BuildHasherDefault».name)
+
+theorem buildHasherDefault_default_spec {p H}
+    {h_hasher : Hasher.hasImpl env H}
+    {h_default : Default.hasDefaultImpl env H}
+    : STHoare p env ⟦⟧
+        (Lampe.Stdlib.Default.default h![] (BuildHasherDefaultTp H) h![] h![] h![])
+        (fun r => r = buildHasherDefaultRepr (H := H)) := by
+  resolve_trait
+  steps
+  simp [buildHasherDefaultRepr, *]
+
+theorem buildHasherDefault_build_hasher_spec {p H}
+    {h_hasher : Hasher.hasImpl env H}
+    {h_default : Default.hasDefaultImpl env H}
+    {h : Tp.denote p H}
+    (h_default_spec : STHoare p env ⟦⟧
+      (Lampe.Stdlib.Default.default h![] H h![] h![] h![])
+      (fun r => r = h))
+    : STHoare p env ⟦⟧
+        («std-1.0.0-beta.14::hash::BuildHasher».build_hasher
+          h![] (BuildHasherDefaultTp H) h![H] h![] h![buildHasherDefaultRepr (H := H)])
+        (fun r => r = h) := by
+  resolve_trait
+  steps [h_default_spec]
+  assumption
+
+theorem field_hash_spec {p H stateRef}
+    {self : Fp p}
+    {state final : Tp.denote p H}
+    {h_hasher : Hasher.hasImpl env H}
+    (h_write_spec : STHoare p env
+      [stateRef ↦ ⟨H, state⟩]
+      («std-1.0.0-beta.14::hash::Hasher».write h![] H h![] h![] h![stateRef, self])
+      (fun _ => [stateRef ↦ ⟨H, final⟩]))
+    : STHoare p env
+        [stateRef ↦ ⟨H, state⟩]
+        («std-1.0.0-beta.14::hash::Hash».hash h![] .field h![] h![H] h![self, stateRef])
+        (fun _ => [stateRef ↦ ⟨H, final⟩]) := by
+  resolve_trait
+  steps [h_write_spec]
+
+theorem u1_hash_spec {p H stateRef}
+    {self : U 1}
+    {state final : Tp.denote p H}
+    {h_hasher : Hasher.hasImpl env H}
+    (h_write_spec : STHoare p env
+      [stateRef ↦ ⟨H, state⟩]
+      («std-1.0.0-beta.14::hash::Hasher».write h![] H h![] h![]
+        h![stateRef, @Builtin.CastTp.cast (.u 1) .field _ p self])
+      (fun _ => [stateRef ↦ ⟨H, final⟩]))
+    : STHoare p env
+        [stateRef ↦ ⟨H, state⟩]
+        («std-1.0.0-beta.14::hash::Hash».hash h![] (.u 1) h![] h![H] h![self, stateRef])
+        (fun _ => [stateRef ↦ ⟨H, final⟩]) := by
+  resolve_trait
+  steps [h_write_spec]
+
+theorem u8_hash_spec {p H stateRef}
+    {self : U 8}
+    {state final : Tp.denote p H}
+    {h_hasher : Hasher.hasImpl env H}
+    (h_write_spec : STHoare p env
+      [stateRef ↦ ⟨H, state⟩]
+      («std-1.0.0-beta.14::hash::Hasher».write h![] H h![] h![]
+        h![stateRef, @Builtin.CastTp.cast (.u 8) .field _ p self])
+      (fun _ => [stateRef ↦ ⟨H, final⟩]))
+    : STHoare p env
+        [stateRef ↦ ⟨H, state⟩]
+        («std-1.0.0-beta.14::hash::Hash».hash h![] (.u 8) h![] h![H] h![self, stateRef])
+        (fun _ => [stateRef ↦ ⟨H, final⟩]) := by
+  resolve_trait
+  steps [h_write_spec]
+
+theorem u16_hash_spec {p H stateRef}
+    {self : U 16}
+    {state final : Tp.denote p H}
+    {h_hasher : Hasher.hasImpl env H}
+    (h_write_spec : STHoare p env
+      [stateRef ↦ ⟨H, state⟩]
+      («std-1.0.0-beta.14::hash::Hasher».write h![] H h![] h![]
+        h![stateRef, @Builtin.CastTp.cast (.u 16) .field _ p self])
+      (fun _ => [stateRef ↦ ⟨H, final⟩]))
+    : STHoare p env
+        [stateRef ↦ ⟨H, state⟩]
+        («std-1.0.0-beta.14::hash::Hash».hash h![] (.u 16) h![] h![H] h![self, stateRef])
+        (fun _ => [stateRef ↦ ⟨H, final⟩]) := by
+  resolve_trait
+  steps [h_write_spec]
+
+theorem u32_hash_spec {p H stateRef}
+    {self : U 32}
+    {state final : Tp.denote p H}
+    {h_hasher : Hasher.hasImpl env H}
+    (h_write_spec : STHoare p env
+      [stateRef ↦ ⟨H, state⟩]
+      («std-1.0.0-beta.14::hash::Hasher».write h![] H h![] h![]
+        h![stateRef, @Builtin.CastTp.cast (.u 32) .field _ p self])
+      (fun _ => [stateRef ↦ ⟨H, final⟩]))
+    : STHoare p env
+        [stateRef ↦ ⟨H, state⟩]
+        («std-1.0.0-beta.14::hash::Hash».hash h![] (.u 32) h![] h![H] h![self, stateRef])
+        (fun _ => [stateRef ↦ ⟨H, final⟩]) := by
+  resolve_trait
+  steps [h_write_spec]
+
+theorem u64_hash_spec {p H stateRef}
+    {self : U 64}
+    {state final : Tp.denote p H}
+    {h_hasher : Hasher.hasImpl env H}
+    (h_write_spec : STHoare p env
+      [stateRef ↦ ⟨H, state⟩]
+      («std-1.0.0-beta.14::hash::Hasher».write h![] H h![] h![]
+        h![stateRef, @Builtin.CastTp.cast (.u 64) .field _ p self])
+      (fun _ => [stateRef ↦ ⟨H, final⟩]))
+    : STHoare p env
+        [stateRef ↦ ⟨H, state⟩]
+        («std-1.0.0-beta.14::hash::Hash».hash h![] (.u 64) h![] h![H] h![self, stateRef])
+        (fun _ => [stateRef ↦ ⟨H, final⟩]) := by
+  resolve_trait
+  steps [h_write_spec]
+
+theorem u128_hash_spec {p H stateRef}
+    {self : U 128}
+    {state final : Tp.denote p H}
+    {h_hasher : Hasher.hasImpl env H}
+    (h_write_spec : STHoare p env
+      [stateRef ↦ ⟨H, state⟩]
+      («std-1.0.0-beta.14::hash::Hasher».write h![] H h![] h![]
+        h![stateRef, @Builtin.CastTp.cast (.u 128) .field _ p self])
+      (fun _ => [stateRef ↦ ⟨H, final⟩]))
+    : STHoare p env
+        [stateRef ↦ ⟨H, state⟩]
+        («std-1.0.0-beta.14::hash::Hash».hash h![] (.u 128) h![] h![H] h![self, stateRef])
+        (fun _ => [stateRef ↦ ⟨H, final⟩]) := by
+  resolve_trait
+  steps [h_write_spec]
+
+theorem i8_hash_spec {p H stateRef}
+    {self : Tp.denote p (.i 8)}
+    {state final : Tp.denote p H}
+    {h_hasher : Hasher.hasImpl env H}
+    (h_write_spec : STHoare p env
+      [stateRef ↦ ⟨H, state⟩]
+      («std-1.0.0-beta.14::hash::Hasher».write h![] H h![] h![]
+        h![stateRef, @Builtin.CastTp.cast (.u 8) .field _ p
+          (@Builtin.CastTp.cast (.i 8) (.u 8) _ p self)])
+      (fun _ => [stateRef ↦ ⟨H, final⟩]))
+    : STHoare p env
+        [stateRef ↦ ⟨H, state⟩]
+        («std-1.0.0-beta.14::hash::Hash».hash h![] (.i 8) h![] h![H] h![self, stateRef])
+        (fun _ => [stateRef ↦ ⟨H, final⟩]) := by
+  resolve_trait
+  steps [h_write_spec]
+
+theorem i16_hash_spec {p H stateRef}
+    {self : Tp.denote p (.i 16)}
+    {state final : Tp.denote p H}
+    {h_hasher : Hasher.hasImpl env H}
+    (h_write_spec : STHoare p env
+      [stateRef ↦ ⟨H, state⟩]
+      («std-1.0.0-beta.14::hash::Hasher».write h![] H h![] h![]
+        h![stateRef, @Builtin.CastTp.cast (.u 16) .field _ p
+          (@Builtin.CastTp.cast (.i 16) (.u 16) _ p self)])
+      (fun _ => [stateRef ↦ ⟨H, final⟩]))
+    : STHoare p env
+        [stateRef ↦ ⟨H, state⟩]
+        («std-1.0.0-beta.14::hash::Hash».hash h![] (.i 16) h![] h![H] h![self, stateRef])
+        (fun _ => [stateRef ↦ ⟨H, final⟩]) := by
+  resolve_trait
+  steps [h_write_spec]
+
+theorem i32_hash_spec {p H stateRef}
+    {self : Tp.denote p (.i 32)}
+    {state final : Tp.denote p H}
+    {h_hasher : Hasher.hasImpl env H}
+    (h_write_spec : STHoare p env
+      [stateRef ↦ ⟨H, state⟩]
+      («std-1.0.0-beta.14::hash::Hasher».write h![] H h![] h![]
+        h![stateRef, @Builtin.CastTp.cast (.u 32) .field _ p
+          (@Builtin.CastTp.cast (.i 32) (.u 32) _ p self)])
+      (fun _ => [stateRef ↦ ⟨H, final⟩]))
+    : STHoare p env
+        [stateRef ↦ ⟨H, state⟩]
+        («std-1.0.0-beta.14::hash::Hash».hash h![] (.i 32) h![] h![H] h![self, stateRef])
+        (fun _ => [stateRef ↦ ⟨H, final⟩]) := by
+  resolve_trait
+  steps [h_write_spec]
+
+theorem i64_hash_spec {p H stateRef}
+    {self : Tp.denote p (.i 64)}
+    {state final : Tp.denote p H}
+    {h_hasher : Hasher.hasImpl env H}
+    (h_write_spec : STHoare p env
+      [stateRef ↦ ⟨H, state⟩]
+      («std-1.0.0-beta.14::hash::Hasher».write h![] H h![] h![]
+        h![stateRef, @Builtin.CastTp.cast (.u 64) .field _ p
+          (@Builtin.CastTp.cast (.i 64) (.u 64) _ p self)])
+      (fun _ => [stateRef ↦ ⟨H, final⟩]))
+    : STHoare p env
+        [stateRef ↦ ⟨H, state⟩]
+        («std-1.0.0-beta.14::hash::Hash».hash h![] (.i 64) h![] h![H] h![self, stateRef])
+        (fun _ => [stateRef ↦ ⟨H, final⟩]) := by
+  resolve_trait
+  steps [h_write_spec]
+
+theorem bool_hash_spec {p H stateRef}
+    {self : Bool}
+    {state final : Tp.denote p H}
+    {h_hasher : Hasher.hasImpl env H}
+    (h_write_spec : STHoare p env
+      [stateRef ↦ ⟨H, state⟩]
+      («std-1.0.0-beta.14::hash::Hasher».write h![] H h![] h![]
+        h![stateRef, @Builtin.CastTp.cast .bool .field _ p self])
+      (fun _ => [stateRef ↦ ⟨H, final⟩]))
+    : STHoare p env
+        [stateRef ↦ ⟨H, state⟩]
+        («std-1.0.0-beta.14::hash::Hash».hash h![] .bool h![] h![H] h![self, stateRef])
+        (fun _ => [stateRef ↦ ⟨H, final⟩]) := by
+  resolve_trait
+  steps [h_write_spec]
+
+theorem unit_hash_spec {p H stateRef}
+    {state : Tp.denote p H}
+    : STHoare p env
+        [stateRef ↦ ⟨H, state⟩]
+        («std-1.0.0-beta.14::hash::Hash».hash h![] .unit h![] h![H] h![(), stateRef])
+        (fun _ => [stateRef ↦ ⟨H, state⟩]) := by
+  resolve_trait
+  steps
